wip dowhile intro

Lang.v
@@ -2,21 +2,27 @@ Require Import Arith Lia List String.
 
 Inductive Expr : Type :=
 | Arg: Expr
-| Single: Expr -> Expr
-| Concat: Expr -> Expr -> Expr
 | Num: nat -> Expr
 | Boolean: bool -> Expr
 | Add: Expr -> Expr -> Expr
 | LessThan: Expr -> Expr -> Expr
+(* Tuples *)
+| Single: Expr -> Expr
+| Concat: Expr -> Expr -> Expr
+| Get : Expr -> nat -> Expr
+(* Effects *)
 | Print : Expr -> Expr -> Expr
-(* pred in then else*)
+| Store : Expr -> Expr -> Expr
+| Load : Expr -> Expr
+(* pred in then else *)
 | If : Expr -> Expr -> Expr -> Expr -> Expr
 (* in pred out *)
 | DoWhile : Expr -> Expr -> Expr -> Expr
-(* pred in e *)
-| CtxInThen : Expr -> Expr -> Expr -> Expr
-(* pred in e *)
-| CtxInElse : Expr -> Expr -> Expr -> Expr
+| Ctx : Assumption -> Expr -> Expr
+with Assumption : Type :=
+| InThen : Expr -> Expr -> Assumption
+| InElse : Expr -> Expr -> Assumption
+| InDoWhile : Expr -> Expr -> Expr -> Assumption
 .
 
 Inductive Typ : Type :=
@@ -41,6 +47,10 @@ Inductive Value : Type :=
 Definition initstate :=
   (VState {| Mem := nil; Log := nil |}).
 
+Inductive nth_element {A : Type} : nat -> list A -> A -> Prop :=
+| nth_zero : forall x l, nth_element 0 (x :: l) x
+| nth_S : forall n x y l, nth_element n l x -> nth_element (S n) (y :: l) x.
+
 (* Big-step judgement *)
 Inductive BS : Value -> Expr -> Value -> Prop :=
 | EArg : forall a,
@@ -57,6 +67,17 @@ Inductive BS : Value -> Expr -> Value -> Prop :=
   BS a e1 (VNum n1) ->
   BS a e2 (VNum n2) ->
   BS a (LessThan e1 e2) (VBoolean (Nat.ltb n1 n2))
+| ESingle : forall a e v,
+  BS a e v ->
+  BS a (Single e) (VTuple (cons v nil))
+| EConcat: forall a e1 e2 t1 t2,
+  BS a e1 (VTuple t1) ->
+  BS a e2 (VTuple t2) ->
+  BS a (Concat e1 e2) (VTuple (t1 ++ t2))
+| EGet: forall a e vs i v,
+  BS a e (VTuple vs) ->
+  nth_element i vs v ->
+  BS a (Get e i) v
 | EPrint : forall a estate mem log e n,
   BS a estate (VState {| Mem := mem; Log := log |}) ->
   BS a e (VNum n) ->
@@ -86,12 +107,25 @@ Inductive BS : Value -> Expr -> Value -> Prop :=
   BS a e v ->
   BS a0 ei a ->
   BS a0 ep (VBoolean true) ->
-  BS a (CtxInThen ep ei e) v
+  BS a (Ctx (InThen ep ei) e) v
 | ECtxInElse : forall a ei ep e v a0,
   BS a e v ->
   BS a0 ei a ->
   BS a0 ep (VBoolean false) ->
-  BS a (CtxInElse ep ei e)v
+  BS a (Ctx (InElse ep ei) e) v
+| ECtxInDoWhile : forall a ei ep eo e v,
+  BS a e v ->
+  WhileProducesArg ei ep eo a ->
+  BS a (Ctx (InDoWhile ei ep eo) e) v
+with WhileProducesArg : Expr -> Expr -> Expr -> Value -> Prop :=
+| InitArg : forall a0 ei ep eo vi,
+  BS a0 ei vi ->
+  WhileProducesArg ei ep eo vi
+| NextArg : forall a ei ep eo vi,
+  WhileProducesArg ei ep eo a ->
+  BS a ep (VBoolean true) ->
+  BS a ei vi ->
+  WhileProducesArg ei ep eo vi
 .
 
 Notation "A ⊢ B ⇓ C" := (BS A B C) (at level 80).
@@ -129,7 +163,7 @@ Qed.
 Theorem introduce_if_ctx : forall a ep ei et ee v,
   a ⊢ If ep ei et ee ⇓ v
   <->
-  a ⊢ If ep ei (CtxInThen ep ei et) (CtxInElse ep ei ee) ⇓ v
+  a ⊢ If ep ei (Ctx (InThen ep ei) et) (Ctx (InElse ep ei) ee) ⇓ v
 .
 Proof.
   split. 
@@ -154,10 +188,101 @@ Proof.
       + inversion H8; auto.
 Qed.
 
-Theorem ctx_allows_const_union : forall a ep n v,
-  a ⊢ CtxInThen ep (Num n) Arg ⇓ v
+Theorem introduce_do_while_ctx : forall ei ep eo,
+  forall a v,
+  a ⊢ DoWhile ei ep eo ⇓ v
+  ->
+  a ⊢ DoWhile ei (Ctx (InDoWhile ei ep eo) ep) (Ctx (InDoWhile ei ep eo) eo) ⇓ v
+.
+Proof.
+  - intros. inversion H. 
+  (* We can prove EDoWhileFalse *)
+  2: {
+    eapply EDoWhileFalse; subst.
+    - apply H4.
+    - apply ECtxInDoWhile.
+      * auto.
+      * eapply InitArg. apply H4.
+    - eapply ECtxInDoWhile.
+      * auto.
+      * eapply InitArg. apply H4.
+  }
+  (* We can prove "one iteration" of EDoWhileTrue *)
+  - eapply EDoWhileTrue; auto.
+    * apply H3.
+    * eapply ECtxInDoWhile; auto. eapply InitArg. apply H3.
+    * eapply ECtxInDoWhile; auto.
+      ** apply H7.
+      ** eapply InitArg. apply H3.
+    * subst.
+    (* But here I think I need induction*)
+Admitted.
+
+Require Import FrapWithoutSets.
+
+(* Let's try again... *)
+Theorem introduce_do_while_ctx2 : forall ei ep eo,
+  forall a v,
+  a ⊢ DoWhile ei ep eo ⇓ v
+  ->
+  a ⊢ DoWhile ei (Ctx (InDoWhile ei ep eo) ep) (Ctx (InDoWhile ei ep eo) eo) ⇓ v
+.
+Proof.
+  intros. induct H.
+  - 
+Admitted.
+
+(* https://stackoverflow.com/questions/55965468/what-to-do-when-the-induction-removes-too-much-information-to-make-the-goal-solv *)
+
+(* Induct from frap *)
+
+  
+  
+  
+   induction H.
+  - 
+  - intros.
+    * induction H.
+      + 
+      + eapply EDoWhileTrue; auto.
+        -- apply H3.
+        -- eapply ECtxInDoWhile; auto. eapply InitArg. apply H3.
+        -- eapply ECtxInDoWhile; auto.
+          ** apply H7.
+          ** eapply InitArg. apply H3.
+        -- eapply EDoWhileTrue; auto.
+
+Theorem introduce_do_while_ctx : forall a ei ep eo v,
+  a ⊢ DoWhile ei ep eo ⇓ v
   <->
-  a ⊢ CtxInThen ep (Num n) (Num n) ⇓ v
+  a ⊢ DoWhile ei (Ctx (InDoWhile ei ep eo) ep) (Ctx (InDoWhile ei ep eo) eo) ⇓ v
+.
+Proof.
+  split. 
+  - intros.
+    * inversion H; subst.
+      + eapply EDoWhileTrue; auto.
+        -- apply H3.
+        -- eapply ECtxInDoWhile; auto. eapply InitArg. apply H3.
+        -- eapply ECtxInDoWhile; auto.
+          ** apply H7.
+          ** eapply InitArg. apply H3.
+        -- eapply EDoWhileTrue; auto.
+
+
+  - intros. inversion H.
+    * eapply EIfTrue; auto.
+      + apply H7.
+      + inversion H8; auto.
+    * eapply EIfFalse; auto.
+      + apply H7.
+      + inversion H8; auto.
+Qed.
+
+Theorem ctx_allows_const_union : forall a ep n v,
+  a ⊢ Ctx (InThen ep (Num n)) Arg ⇓ v
+  <->
+  a ⊢ Ctx (InThen ep (Num n)) (Num n) ⇓ v
 .
 Proof.
   split.
@@ -172,3 +297,41 @@ Proof.
       + subst. inversion H6. subst. inversion H4. subst. apply ENum.
       + subst. apply H7. 
 Qed.
+
+Fixpoint subst (e: Expr) (newctx : Assumption) (v : Expr) :=
+  match e with
+  | Arg => v
+  | Single e1 => Single (subst e1 newctx v)
+  | Concat e1 e2 => Concat (subst e1 newctx v) (subst e2 newctx v)
+  | Boolean b => Boolean b
+  | Num n => Num n
+  | Add e1 e2 => Add (subst e1 newctx v) (subst e2 newctx v)
+  | LessThan e1 e2 => LessThan (subst e1 newctx v) (subst e2 newctx v)
+  | Print e1 e2 => Print (subst e1 newctx v) (subst e2 newctx v)
+  | If p i t e => If (subst p newctx v) (subst i newctx v) t e
+  | DoWhile ei ep eo => DoWhile (subst ei newctx v) ep eo
+  | Ctx ctx e => Ctx newctx (subst e newctx v)
+  end.
+(* 
+Theorem subst_lemma : forall a a0 e v ea newctx,
+a0 ⊢ ea ⇓ a /\ a0 ⊢ subst e newctx ea ⇓ v
+->
+a ⊢ e ⇓ v
+.
+Proof.
+  intros. destruct H. *)
+
+
+(* 
+Theorem in_then_allows_pred_true_union : forall a ep ei v newctx,
+  a ⊢ Ctx (InThen (subst ep newctx ei) ei) ep ⇓ v
+  <->
+  a ⊢ Ctx (InThen (subst ep newctx ei) ei) (Boolean true) ⇓ v
+.
+Proof.
+  split.
+  - intros. eapply ECtxInThen.
+    * inversion H. subst. inversion H7; subst. *)
+
+(* need subst_lemma and lang_deterministic *)
+  
